theories/AutoSubst/Ast.v
@@ -9,7 +9,7 @@ Inductive term : Type :=
   | tRel : nat -> term
   | tSort : sort -> term
   | tProd : term -> term -> term
-  | tLambda : term -> term -> term
+  | tLambda : option (term) -> term -> term
   | tApp : term -> term -> term
   | tNat : term
   | tZero : term
@@ -35,8 +35,8 @@ exact (eq_trans (eq_trans eq_refl (ap (fun x => tProd x s1) H0))
          (ap (fun x => tProd t0 x) H1)).
 Qed.
 
-Lemma congr_tLambda {s0 : term} {s1 : term} {t0 : term} {t1 : term}
-  (H0 : s0 = t0) (H1 : s1 = t1) : tLambda s0 s1 = tLambda t0 t1.
+Lemma congr_tLambda {s0 : option (term)} {s1 : term} {t0 : option (term)}
+  {t1 : term} (H0 : s0 = t0) (H1 : s1 = t1) : tLambda s0 s1 = tLambda t0 t1.
 Proof.
 exact (eq_trans (eq_trans eq_refl (ap (fun x => tLambda x s1) H0))
          (ap (fun x => tLambda t0 x) H1)).
@@ -132,7 +132,8 @@ Fixpoint ren_term (xi_term : nat -> nat) (s : term) {struct s} : term :=
   | tProd s0 s1 =>
       tProd (ren_term xi_term s0) (ren_term (upRen_term_term xi_term) s1)
   | tLambda s0 s1 =>
-      tLambda (ren_term xi_term s0) (ren_term (upRen_term_term xi_term) s1)
+      tLambda (option_map (ren_term xi_term) s0)
+        (ren_term (upRen_term_term xi_term) s1)
   | tApp s0 s1 => tApp (ren_term xi_term s0) (ren_term xi_term s1)
   | tNat => tNat
   | tZero => tZero
@@ -167,7 +168,7 @@ term :=
       tProd (subst_term sigma_term s0)
         (subst_term (up_term_term sigma_term) s1)
   | tLambda s0 s1 =>
-      tLambda (subst_term sigma_term s0)
+      tLambda (option_map (subst_term sigma_term) s0)
         (subst_term (up_term_term sigma_term) s1)
   | tApp s0 s1 => tApp (subst_term sigma_term s0) (subst_term sigma_term s1)
   | tNat => tNat
@@ -212,7 +213,7 @@ subst_term sigma_term s = s :=
       congr_tProd (idSubst_term sigma_term Eq_term s0)
         (idSubst_term (up_term_term sigma_term) (upId_term_term _ Eq_term) s1)
   | tLambda s0 s1 =>
-      congr_tLambda (idSubst_term sigma_term Eq_term s0)
+      congr_tLambda (option_id (idSubst_term sigma_term Eq_term) s0)
         (idSubst_term (up_term_term sigma_term) (upId_term_term _ Eq_term) s1)
   | tApp s0 s1 =>
       congr_tApp (idSubst_term sigma_term Eq_term s0)
@@ -264,7 +265,7 @@ ren_term xi_term s = ren_term zeta_term s :=
         (extRen_term (upRen_term_term xi_term) (upRen_term_term zeta_term)
            (upExtRen_term_term _ _ Eq_term) s1)
   | tLambda s0 s1 =>
-      congr_tLambda (extRen_term xi_term zeta_term Eq_term s0)
+      congr_tLambda (option_ext (extRen_term xi_term zeta_term Eq_term) s0)
         (extRen_term (upRen_term_term xi_term) (upRen_term_term zeta_term)
            (upExtRen_term_term _ _ Eq_term) s1)
   | tApp s0 s1 =>
@@ -322,7 +323,7 @@ subst_term sigma_term s = subst_term tau_term s :=
         (ext_term (up_term_term sigma_term) (up_term_term tau_term)
            (upExt_term_term _ _ Eq_term) s1)
   | tLambda s0 s1 =>
-      congr_tLambda (ext_term sigma_term tau_term Eq_term s0)
+      congr_tLambda (option_ext (ext_term sigma_term tau_term Eq_term) s0)
         (ext_term (up_term_term sigma_term) (up_term_term tau_term)
            (upExt_term_term _ _ Eq_term) s1)
   | tApp s0 s1 =>
@@ -380,7 +381,8 @@ Fixpoint compRenRen_term (xi_term : nat -> nat) (zeta_term : nat -> nat)
            (upRen_term_term zeta_term) (upRen_term_term rho_term)
            (up_ren_ren _ _ _ Eq_term) s1)
   | tLambda s0 s1 =>
-      congr_tLambda (compRenRen_term xi_term zeta_term rho_term Eq_term s0)
+      congr_tLambda
+        (option_comp (compRenRen_term xi_term zeta_term rho_term Eq_term) s0)
         (compRenRen_term (upRen_term_term xi_term)
            (upRen_term_term zeta_term) (upRen_term_term rho_term)
            (up_ren_ren _ _ _ Eq_term) s1)
@@ -451,7 +453,8 @@ subst_term tau_term (ren_term xi_term s) = subst_term theta_term s :=
            s1)
   | tLambda s0 s1 =>
       congr_tLambda
-        (compRenSubst_term xi_term tau_term theta_term Eq_term s0)
+        (option_comp (compRenSubst_term xi_term tau_term theta_term Eq_term)
+           s0)
         (compRenSubst_term (upRen_term_term xi_term) (up_term_term tau_term)
            (up_term_term theta_term) (up_ren_subst_term_term _ _ _ Eq_term)
            s1)
@@ -530,7 +533,8 @@ ren_term zeta_term (subst_term sigma_term s) = subst_term theta_term s :=
            (up_subst_ren_term_term _ _ _ Eq_term) s1)
   | tLambda s0 s1 =>
       congr_tLambda
-        (compSubstRen_term sigma_term zeta_term theta_term Eq_term s0)
+        (option_comp
+           (compSubstRen_term sigma_term zeta_term theta_term Eq_term) s0)
         (compSubstRen_term (up_term_term sigma_term)
            (upRen_term_term zeta_term) (up_term_term theta_term)
            (up_subst_ren_term_term _ _ _ Eq_term) s1)
@@ -620,7 +624,8 @@ subst_term tau_term (subst_term sigma_term s) = subst_term theta_term s :=
            (up_subst_subst_term_term _ _ _ Eq_term) s1)
   | tLambda s0 s1 =>
       congr_tLambda
-        (compSubstSubst_term sigma_term tau_term theta_term Eq_term s0)
+        (option_comp
+           (compSubstSubst_term sigma_term tau_term theta_term Eq_term) s0)
         (compSubstSubst_term (up_term_term sigma_term)
            (up_term_term tau_term) (up_term_term theta_term)
            (up_subst_subst_term_term _ _ _ Eq_term) s1)
@@ -759,7 +764,8 @@ Fixpoint rinst_inst_term (xi_term : nat -> nat) (sigma_term : nat -> term)
         (rinst_inst_term (upRen_term_term xi_term) (up_term_term sigma_term)
            (rinstInst_up_term_term _ _ Eq_term) s1)
   | tLambda s0 s1 =>
-      congr_tLambda (rinst_inst_term xi_term sigma_term Eq_term s0)
+      congr_tLambda
+        (option_ext (rinst_inst_term xi_term sigma_term Eq_term) s0)
         (rinst_inst_term (upRen_term_term xi_term) (up_term_term sigma_term)
            (rinstInst_up_term_term _ _ Eq_term) s1)
   | tApp s0 s1 =>
@@ -857,13 +863,13 @@ Qed.
 Class Up_term X Y :=
     up_term : X -> Y.
 
-#[global] Instance Subst_term : (Subst1 _ _ _) := @subst_term.
+#[global]Instance Subst_term : (Subst1 _ _ _) := @subst_term.
 
-#[global] Instance Up_term_term : (Up_term _ _) := @up_term_term.
+#[global]Instance Up_term_term : (Up_term _ _) := @up_term_term.
 
-#[global] Instance Ren_term : (Ren1 _ _ _) := @ren_term.
+#[global]Instance Ren_term : (Ren1 _ _ _) := @ren_term.
 
-#[global] Instance VarInstance_term : (Var _ _) := @tRel.
+#[global]Instance VarInstance_term : (Var _ _) := @tRel.
 
 Notation "[ sigma_term ]" := (subst_term sigma_term)
   ( at level 1, left associativity, only printing) : fscope.
@@ -889,7 +895,7 @@ Notation "x '__term'" := (@ids _ _ VarInstance_term x)
 Notation "x '__term'" := (tRel x) ( at level 5, format "x __term") :
   subst_scope.
 
-#[global] Instance subst_term_morphism :
+#[global]Instance subst_term_morphism :
  (Proper (respectful (pointwise_relation _ eq) (respectful eq eq))
     (@subst_term)).
 Proof.
@@ -898,14 +904,14 @@ exact (fun f_term g_term Eq_term s t Eq_st =>
          (ext_term f_term g_term Eq_term s) t Eq_st).
 Qed.
 
-#[global] Instance subst_term_morphism2 :
+#[global]Instance subst_term_morphism2 :
  (Proper (respectful (pointwise_relation _ eq) (pointwise_relation _ eq))
     (@subst_term)).
 Proof.
 exact (fun f_term g_term Eq_term s => ext_term f_term g_term Eq_term s).
 Qed.
 
-#[global] Instance ren_term_morphism :
+#[global]Instance ren_term_morphism :
  (Proper (respectful (pointwise_relation _ eq) (respectful eq eq))
     (@ren_term)).
 Proof.
@@ -914,7 +920,7 @@ exact (fun f_term g_term Eq_term s t Eq_st =>
          (extRen_term f_term g_term Eq_term s) t Eq_st).
 Qed.
 
-#[global] Instance ren_term_morphism2 :
+#[global]Instance ren_term_morphism2 :
  (Proper (respectful (pointwise_relation _ eq) (pointwise_relation _ eq))
     (@ren_term)).
 Proof.
@@ -973,687 +979,6 @@ Ltac renamify := auto_unfold;
 
 End Core.
 
-Module Allfv.
-
-Import
-Core.
-
-Lemma upAllfv_term_term (p : nat -> Prop) : nat -> Prop.
-Proof.
-exact (up_allfv p).
-Defined.
-
-Fixpoint allfv_term (p_term : nat -> Prop) (s : term) {struct s} : Prop :=
-  match s with
-  | tRel s0 => p_term s0
-  | tSort s0 => and True True
-  | tProd s0 s1 =>
-      and (allfv_term p_term s0)
-        (and (allfv_term (upAllfv_term_term p_term) s1) True)
-  | tLambda s0 s1 =>
-      and (allfv_term p_term s0)
-        (and (allfv_term (upAllfv_term_term p_term) s1) True)
-  | tApp s0 s1 =>
-      and (allfv_term p_term s0) (and (allfv_term p_term s1) True)
-  | tNat => True
-  | tZero => True
-  | tSucc s0 => and (allfv_term p_term s0) True
-  | tNatElim s0 s1 s2 s3 =>
-      and (allfv_term (upAllfv_term_term p_term) s0)
-        (and (allfv_term p_term s1)
-           (and (allfv_term p_term s2) (and (allfv_term p_term s3) True)))
-  | tEmpty => True
-  | tEmptyElim s0 s1 =>
-      and (allfv_term (upAllfv_term_term p_term) s0)
-        (and (allfv_term p_term s1) True)
-  | tSig s0 s1 =>
-      and (allfv_term p_term s0)
-        (and (allfv_term (upAllfv_term_term p_term) s1) True)
-  | tPair s0 s1 s2 s3 =>
-      and (allfv_term p_term s0)
-        (and (allfv_term (upAllfv_term_term p_term) s1)
-           (and (allfv_term p_term s2) (and (allfv_term p_term s3) True)))
-  | tFst s0 => and (allfv_term p_term s0) True
-  | tSnd s0 => and (allfv_term p_term s0) True
-  end.
-
-Lemma upAllfvTriv_term_term {p : nat -> Prop} (H : forall x, p x) :
-  forall x, upAllfv_term_term p x.
-Proof.
-exact (fun x => match x with
-                | S n' => H n'
-                | O => I
-                end).
-Qed.
-
-Fixpoint allfvTriv_term (p_term : nat -> Prop) (H_term : forall x, p_term x)
-(s : term) {struct s} : allfv_term p_term s :=
-  match s with
-  | tRel s0 => H_term s0
-  | tSort s0 => conj I I
-  | tProd s0 s1 =>
-      conj (allfvTriv_term p_term H_term s0)
-        (conj
-           (allfvTriv_term (upAllfv_term_term p_term)
-              (upAllfvTriv_term_term H_term) s1) I)
-  | tLambda s0 s1 =>
-      conj (allfvTriv_term p_term H_term s0)
-        (conj
-           (allfvTriv_term (upAllfv_term_term p_term)
-              (upAllfvTriv_term_term H_term) s1) I)
-  | tApp s0 s1 =>
-      conj (allfvTriv_term p_term H_term s0)
-        (conj (allfvTriv_term p_term H_term s1) I)
-  | tNat => I
-  | tZero => I
-  | tSucc s0 => conj (allfvTriv_term p_term H_term s0) I
-  | tNatElim s0 s1 s2 s3 =>
-      conj
-        (allfvTriv_term (upAllfv_term_term p_term)
-           (upAllfvTriv_term_term H_term) s0)
-        (conj (allfvTriv_term p_term H_term s1)
-           (conj (allfvTriv_term p_term H_term s2)
-              (conj (allfvTriv_term p_term H_term s3) I)))
-  | tEmpty => I
-  | tEmptyElim s0 s1 =>
-      conj
-        (allfvTriv_term (upAllfv_term_term p_term)
-           (upAllfvTriv_term_term H_term) s0)
-        (conj (allfvTriv_term p_term H_term s1) I)
-  | tSig s0 s1 =>
-      conj (allfvTriv_term p_term H_term s0)
-        (conj
-           (allfvTriv_term (upAllfv_term_term p_term)
-              (upAllfvTriv_term_term H_term) s1) I)
-  | tPair s0 s1 s2 s3 =>
-      conj (allfvTriv_term p_term H_term s0)
-        (conj
-           (allfvTriv_term (upAllfv_term_term p_term)
-              (upAllfvTriv_term_term H_term) s1)
-           (conj (allfvTriv_term p_term H_term s2)
-              (conj (allfvTriv_term p_term H_term s3) I)))
-  | tFst s0 => conj (allfvTriv_term p_term H_term s0) I
-  | tSnd s0 => conj (allfvTriv_term p_term H_term s0) I
-  end.
-
-Lemma upAllfvImpl_term_term {p : nat -> Prop} {q : nat -> Prop}
-  (H : forall x, p x -> q x) :
-  forall x, upAllfv_term_term p x -> upAllfv_term_term q x.
-Proof.
-exact (fun x => match x with
-                | S n' => H n'
-                | O => fun Hp => Hp
-                end).
-Qed.
-
-Fixpoint allfvImpl_term (p_term : nat -> Prop) (q_term : nat -> Prop)
-(H_term : forall x, p_term x -> q_term x) (s : term) {struct s} :
-allfv_term p_term s -> allfv_term q_term s :=
-  match s with
-  | tRel s0 => fun HP => H_term s0 HP
-  | tSort s0 => fun HP => conj I I
-  | tProd s0 s1 =>
-      fun HP =>
-      conj
-        (allfvImpl_term p_term q_term H_term s0
-           match HP with
-           | conj HP _ => HP
-           end)
-        (conj
-           (allfvImpl_term (upAllfv_term_term p_term)
-              (upAllfv_term_term q_term) (upAllfvImpl_term_term H_term) s1
-              match HP with
-              | conj _ HP => match HP with
-                             | conj HP _ => HP
-                             end
-              end) I)
-  | tLambda s0 s1 =>
-      fun HP =>
-      conj
-        (allfvImpl_term p_term q_term H_term s0
-           match HP with
-           | conj HP _ => HP
-           end)
-        (conj
-           (allfvImpl_term (upAllfv_term_term p_term)
-              (upAllfv_term_term q_term) (upAllfvImpl_term_term H_term) s1
-              match HP with
-              | conj _ HP => match HP with
-                             | conj HP _ => HP
-                             end
-              end) I)
-  | tApp s0 s1 =>
-      fun HP =>
-      conj
-        (allfvImpl_term p_term q_term H_term s0
-           match HP with
-           | conj HP _ => HP
-           end)
-        (conj
-           (allfvImpl_term p_term q_term H_term s1
-              match HP with
-              | conj _ HP => match HP with
-                             | conj HP _ => HP
-                             end
-              end) I)
-  | tNat => fun HP => I
-  | tZero => fun HP => I
-  | tSucc s0 =>
-      fun HP =>
-      conj
-        (allfvImpl_term p_term q_term H_term s0
-           match HP with
-           | conj HP _ => HP
-           end) I
-  | tNatElim s0 s1 s2 s3 =>
-      fun HP =>
-      conj
-        (allfvImpl_term (upAllfv_term_term p_term) (upAllfv_term_term q_term)
-           (upAllfvImpl_term_term H_term) s0
-           match HP with
-           | conj HP _ => HP
-           end)
-        (conj
-           (allfvImpl_term p_term q_term H_term s1
-              match HP with
-              | conj _ HP => match HP with
-                             | conj HP _ => HP
-                             end
-              end)
-           (conj
-              (allfvImpl_term p_term q_term H_term s2
-                 match HP with
-                 | conj _ HP =>
-                     match HP with
-                     | conj _ HP => match HP with
-                                    | conj HP _ => HP
-                                    end
-                     end
-                 end)
-              (conj
-                 (allfvImpl_term p_term q_term H_term s3
-                    match HP with
-                    | conj _ HP =>
-                        match HP with
-                        | conj _ HP =>
-                            match HP with
-                            | conj _ HP =>
-                                match HP with
-                                | conj HP _ => HP
-                                end
-                            end
-                        end
-                    end) I)))
-  | tEmpty => fun HP => I
-  | tEmptyElim s0 s1 =>
-      fun HP =>
-      conj
-        (allfvImpl_term (upAllfv_term_term p_term) (upAllfv_term_term q_term)
-           (upAllfvImpl_term_term H_term) s0
-           match HP with
-           | conj HP _ => HP
-           end)
-        (conj
-           (allfvImpl_term p_term q_term H_term s1
-              match HP with
-              | conj _ HP => match HP with
-                             | conj HP _ => HP
-                             end
-              end) I)
-  | tSig s0 s1 =>
-      fun HP =>
-      conj
-        (allfvImpl_term p_term q_term H_term s0
-           match HP with
-           | conj HP _ => HP
-           end)
-        (conj
-           (allfvImpl_term (upAllfv_term_term p_term)
-              (upAllfv_term_term q_term) (upAllfvImpl_term_term H_term) s1
-              match HP with
-              | conj _ HP => match HP with
-                             | conj HP _ => HP
-                             end
-              end) I)
-  | tPair s0 s1 s2 s3 =>
-      fun HP =>
-      conj
-        (allfvImpl_term p_term q_term H_term s0
-           match HP with
-           | conj HP _ => HP
-           end)
-        (conj
-           (allfvImpl_term (upAllfv_term_term p_term)
-              (upAllfv_term_term q_term) (upAllfvImpl_term_term H_term) s1
-              match HP with
-              | conj _ HP => match HP with
-                             | conj HP _ => HP
-                             end
-              end)
-           (conj
-              (allfvImpl_term p_term q_term H_term s2
-                 match HP with
-                 | conj _ HP =>
-                     match HP with
-                     | conj _ HP => match HP with
-                                    | conj HP _ => HP
-                                    end
-                     end
-                 end)
-              (conj
-                 (allfvImpl_term p_term q_term H_term s3
-                    match HP with
-                    | conj _ HP =>
-                        match HP with
-                        | conj _ HP =>
-                            match HP with
-                            | conj _ HP =>
-                                match HP with
-                                | conj HP _ => HP
-                                end
-                            end
-                        end
-                    end) I)))
-  | tFst s0 =>
-      fun HP =>
-      conj
-        (allfvImpl_term p_term q_term H_term s0
-           match HP with
-           | conj HP _ => HP
-           end) I
-  | tSnd s0 =>
-      fun HP =>
-      conj
-        (allfvImpl_term p_term q_term H_term s0
-           match HP with
-           | conj HP _ => HP
-           end) I
-  end.
-
-Lemma upAllfvRenL_term_term (p : nat -> Prop) (xi : nat -> nat) :
-  forall x,
-  upAllfv_term_term p (upRen_term_term xi x) ->
-  upAllfv_term_term (funcomp p xi) x.
-Proof.
-exact (fun x => match x with
-                | S n' => fun i => i
-                | O => fun H => H
-                end).
-Qed.
-
-Fixpoint allfvRenL_term (p_term : nat -> Prop) (xi_term : nat -> nat)
-(s : term) {struct s} :
-allfv_term p_term (ren_term xi_term s) ->
-allfv_term (funcomp p_term xi_term) s :=
-  match s with
-  | tRel s0 => fun H => H
-  | tSort s0 => fun H => conj I I
-  | tProd s0 s1 =>
-      fun H =>
-      conj
-        (allfvRenL_term p_term xi_term s0 match H with
-                                          | conj H _ => H
-                                          end)
-        (conj
-           (allfvImpl_term _ _ (upAllfvRenL_term_term p_term xi_term) s1
-              (allfvRenL_term (upAllfv_term_term p_term)
-                 (upRen_term_term xi_term) s1
-                 match H with
-                 | conj _ H => match H with
-                               | conj H _ => H
-                               end
-                 end)) I)
-  | tLambda s0 s1 =>
-      fun H =>
-      conj
-        (allfvRenL_term p_term xi_term s0 match H with
-                                          | conj H _ => H
-                                          end)
-        (conj
-           (allfvImpl_term _ _ (upAllfvRenL_term_term p_term xi_term) s1
-              (allfvRenL_term (upAllfv_term_term p_term)
-                 (upRen_term_term xi_term) s1
-                 match H with
-                 | conj _ H => match H with
-                               | conj H _ => H
-                               end
-                 end)) I)
-  | tApp s0 s1 =>
-      fun H =>
-      conj
-        (allfvRenL_term p_term xi_term s0 match H with
-                                          | conj H _ => H
-                                          end)
-        (conj
-           (allfvRenL_term p_term xi_term s1
-              match H with
-              | conj _ H => match H with
-                            | conj H _ => H
-                            end
-              end) I)
-  | tNat => fun H => I
-  | tZero => fun H => I
-  | tSucc s0 =>
-      fun H =>
-      conj
-        (allfvRenL_term p_term xi_term s0 match H with
-                                          | conj H _ => H
-                                          end) I
-  | tNatElim s0 s1 s2 s3 =>
-      fun H =>
-      conj
-        (allfvImpl_term _ _ (upAllfvRenL_term_term p_term xi_term) s0
-           (allfvRenL_term (upAllfv_term_term p_term)
-              (upRen_term_term xi_term) s0 match H with
-                                           | conj H _ => H
-                                           end))
-        (conj
-           (allfvRenL_term p_term xi_term s1
-              match H with
-              | conj _ H => match H with
-                            | conj H _ => H
-                            end
-              end)
-           (conj
-              (allfvRenL_term p_term xi_term s2
-                 match H with
-                 | conj _ H =>
-                     match H with
-                     | conj _ H => match H with
-                                   | conj H _ => H
-                                   end
-                     end
-                 end)
-              (conj
-                 (allfvRenL_term p_term xi_term s3
-                    match H with
-                    | conj _ H =>
-                        match H with
-                        | conj _ H =>
-                            match H with
-                            | conj _ H => match H with
-                                          | conj H _ => H
-                                          end
-                            end
-                        end
-                    end) I)))
-  | tEmpty => fun H => I
-  | tEmptyElim s0 s1 =>
-      fun H =>
-      conj
-        (allfvImpl_term _ _ (upAllfvRenL_term_term p_term xi_term) s0
-           (allfvRenL_term (upAllfv_term_term p_term)
-              (upRen_term_term xi_term) s0 match H with
-                                           | conj H _ => H
-                                           end))
-        (conj
-           (allfvRenL_term p_term xi_term s1
-              match H with
-              | conj _ H => match H with
-                            | conj H _ => H
-                            end
-              end) I)
-  | tSig s0 s1 =>
-      fun H =>
-      conj
-        (allfvRenL_term p_term xi_term s0 match H with
-                                          | conj H _ => H
-                                          end)
-        (conj
-           (allfvImpl_term _ _ (upAllfvRenL_term_term p_term xi_term) s1
-              (allfvRenL_term (upAllfv_term_term p_term)
-                 (upRen_term_term xi_term) s1
-                 match H with
-                 | conj _ H => match H with
-                               | conj H _ => H
-                               end
-                 end)) I)
-  | tPair s0 s1 s2 s3 =>
-      fun H =>
-      conj
-        (allfvRenL_term p_term xi_term s0 match H with
-                                          | conj H _ => H
-                                          end)
-        (conj
-           (allfvImpl_term _ _ (upAllfvRenL_term_term p_term xi_term) s1
-              (allfvRenL_term (upAllfv_term_term p_term)
-                 (upRen_term_term xi_term) s1
-                 match H with
-                 | conj _ H => match H with
-                               | conj H _ => H
-                               end
-                 end))
-           (conj
-              (allfvRenL_term p_term xi_term s2
-                 match H with
-                 | conj _ H =>
-                     match H with
-                     | conj _ H => match H with
-                                   | conj H _ => H
-                                   end
-                     end
-                 end)
-              (conj
-                 (allfvRenL_term p_term xi_term s3
-                    match H with
-                    | conj _ H =>
-                        match H with
-                        | conj _ H =>
-                            match H with
-                            | conj _ H => match H with
-                                          | conj H _ => H
-                                          end
-                            end
-                        end
-                    end) I)))
-  | tFst s0 =>
-      fun H =>
-      conj
-        (allfvRenL_term p_term xi_term s0 match H with
-                                          | conj H _ => H
-                                          end) I
-  | tSnd s0 =>
-      fun H =>
-      conj
-        (allfvRenL_term p_term xi_term s0 match H with
-                                          | conj H _ => H
-                                          end) I
-  end.
-
-Lemma upAllfvRenR_term_term (p : nat -> Prop) (xi : nat -> nat) :
-  forall x,
-  upAllfv_term_term (funcomp p xi) x ->
-  upAllfv_term_term p (upRen_term_term xi x).
-Proof.
-exact (fun x => match x with
-                | S n' => fun i => i
-                | O => fun H => H
-                end).
-Qed.
-
-Fixpoint allfvRenR_term (p_term : nat -> Prop) (xi_term : nat -> nat)
-(s : term) {struct s} :
-allfv_term (funcomp p_term xi_term) s ->
-allfv_term p_term (ren_term xi_term s) :=
-  match s with
-  | tRel s0 => fun H => H
-  | tSort s0 => fun H => conj I I
-  | tProd s0 s1 =>
-      fun H =>
-      conj
-        (allfvRenR_term p_term xi_term s0 match H with
-                                          | conj H _ => H
-                                          end)
-        (conj
-           (allfvRenR_term (upAllfv_term_term p_term)
-              (upRen_term_term xi_term) s1
-              (allfvImpl_term _ _ (upAllfvRenR_term_term p_term xi_term) s1
-                 match H with
-                 | conj _ H => match H with
-                               | conj H _ => H
-                               end
-                 end)) I)
-  | tLambda s0 s1 =>
-      fun H =>
-      conj
-        (allfvRenR_term p_term xi_term s0 match H with
-                                          | conj H _ => H
-                                          end)
-        (conj
-           (allfvRenR_term (upAllfv_term_term p_term)
-              (upRen_term_term xi_term) s1
-              (allfvImpl_term _ _ (upAllfvRenR_term_term p_term xi_term) s1
-                 match H with
-                 | conj _ H => match H with
-                               | conj H _ => H
-                               end
-                 end)) I)
-  | tApp s0 s1 =>
-      fun H =>
-      conj
-        (allfvRenR_term p_term xi_term s0 match H with
-                                          | conj H _ => H
-                                          end)
-        (conj
-           (allfvRenR_term p_term xi_term s1
-              match H with
-              | conj _ H => match H with
-                            | conj H _ => H
-                            end
-              end) I)
-  | tNat => fun H => I
-  | tZero => fun H => I
-  | tSucc s0 =>
-      fun H =>
-      conj
-        (allfvRenR_term p_term xi_term s0 match H with
-                                          | conj H _ => H
-                                          end) I
-  | tNatElim s0 s1 s2 s3 =>
-      fun H =>
-      conj
-        (allfvRenR_term (upAllfv_term_term p_term) (upRen_term_term xi_term)
-           s0
-           (allfvImpl_term _ _ (upAllfvRenR_term_term p_term xi_term) s0
-              match H with
-              | conj H _ => H
-              end))
-        (conj
-           (allfvRenR_term p_term xi_term s1
-              match H with
-              | conj _ H => match H with
-                            | conj H _ => H
-                            end
-              end)
-           (conj
-              (allfvRenR_term p_term xi_term s2
-                 match H with
-                 | conj _ H =>
-                     match H with
-                     | conj _ H => match H with
-                                   | conj H _ => H
-                                   end
-                     end
-                 end)
-              (conj
-                 (allfvRenR_term p_term xi_term s3
-                    match H with
-                    | conj _ H =>
-                        match H with
-                        | conj _ H =>
-                            match H with
-                            | conj _ H => match H with
-                                          | conj H _ => H
-                                          end
-                            end
-                        end
-                    end) I)))
-  | tEmpty => fun H => I
-  | tEmptyElim s0 s1 =>
-      fun H =>
-      conj
-        (allfvRenR_term (upAllfv_term_term p_term) (upRen_term_term xi_term)
-           s0
-           (allfvImpl_term _ _ (upAllfvRenR_term_term p_term xi_term) s0
-              match H with
-              | conj H _ => H
-              end))
-        (conj
-           (allfvRenR_term p_term xi_term s1
-              match H with
-              | conj _ H => match H with
-                            | conj H _ => H
-                            end
-              end) I)
-  | tSig s0 s1 =>
-      fun H =>
-      conj
-        (allfvRenR_term p_term xi_term s0 match H with
-                                          | conj H _ => H
-                                          end)
-        (conj
-           (allfvRenR_term (upAllfv_term_term p_term)
-              (upRen_term_term xi_term) s1
-              (allfvImpl_term _ _ (upAllfvRenR_term_term p_term xi_term) s1
-                 match H with
-                 | conj _ H => match H with
-                               | conj H _ => H
-                               end
-                 end)) I)
-  | tPair s0 s1 s2 s3 =>
-      fun H =>
-      conj
-        (allfvRenR_term p_term xi_term s0 match H with
-                                          | conj H _ => H
-                                          end)
-        (conj
-           (allfvRenR_term (upAllfv_term_term p_term)
-              (upRen_term_term xi_term) s1
-              (allfvImpl_term _ _ (upAllfvRenR_term_term p_term xi_term) s1
-                 match H with
-                 | conj _ H => match H with
-                               | conj H _ => H
-                               end
-                 end))
-           (conj
-              (allfvRenR_term p_term xi_term s2
-                 match H with
-                 | conj _ H =>
-                     match H with
-                     | conj _ H => match H with
-                                   | conj H _ => H
-                                   end
-                     end
-                 end)
-              (conj
-                 (allfvRenR_term p_term xi_term s3
-                    match H with
-                    | conj _ H =>
-                        match H with
-                        | conj _ H =>
-                            match H with
-                            | conj _ H => match H with
-                                          | conj H _ => H
-                                          end
-                            end
-                        end
-                    end) I)))
-  | tFst s0 =>
-      fun H =>
-      conj
-        (allfvRenR_term p_term xi_term s0 match H with
-                                          | conj H _ => H
-                                          end) I
-  | tSnd s0 =>
-      fun H =>
-      conj
-        (allfvRenR_term p_term xi_term s0 match H with
-                                          | conj H _ => H
-                                          end) I
-  end.
-
-End Allfv.
-
 Module Extra.
 
 Import Core.
@@ -1667,8 +992,6 @@ End Extra.
 Module interface.
 
 Export Core.
-
-Export Allfv.
 
 Export Extra.
 
